src/Log.v
@@ -1,0 +1,40 @@
+Require Import
+  Coq.Unicode.Utf8
+  Coq.Program.Program
+  Coq.Classes.CRelationClasses
+  Coq.Classes.Morphisms
+  Ty
+  Exp
+  Sub.
+
+From Equations Require Import Equations.
+
+Generalizable All Variables.
+
+Section Log.
+
+Context {A : Type}.
+Context `{L : HostExprs A}.
+Context {Γ : Env}.
+
+Variable P : ∀ {τ}, Exp Γ τ → Prop.
+
+(** [ExpP] is a logical predicate that permits type-directed induction on
+    expressions. *)
+Equations ExpP `(e : Exp Γ τ) : Prop :=
+  ExpP (τ:=_ ⟶ _)   f := P f ∧ (∀ x, ExpP x → ExpP (APP f x));
+  ExpP (τ:=_ × _)    p := P p ∧ ExpP (Fst p) ∧ ExpP (Snd p);
+  (* ExpP (τ:=TyList _) l := P l ∧ (∀ d, ExpP d → ExpP (Car d l)); *)
+  ExpP e := P e.
+
+Inductive SubP : ∀ {Γ'}, Sub Γ Γ' → Prop :=
+  | NoSubP : SubP (NoSub (Γ:=Γ))
+  | PushP {Γ' τ} (e : Exp Γ τ) (s : Sub Γ Γ') :
+    ExpP e → SubP s → SubP (Push e s).
+
+Derive Signature for SubP.
+
+Lemma ExpP_P {τ} {e : Γ ⊢ τ} : ExpP e → P e.
+Proof. intros; induction τ; simpl in *; simp ExpP in H; now reduce. Qed.
+
+End Log.
