src/Pat.v
@@ -1,0 +1,24 @@
+Require Export
+  Ty
+  Coq.Lists.List
+  Exp.
+
+From Equations Require Import Equations.
+
+Generalizable All Variables.
+
+Section Pat.
+
+Import ListNotations.
+
+Context {A : Type}.
+Context `{HostExprs A}.
+
+Open Scope Ty_scope.
+
+Inductive Pat : Env → Ty → Type :=
+  | PPair {Γ Γ' τ1 τ2}  : Pat Γ τ1 → Pat Γ' τ2 → Pat (Γ ++ Γ') (TyPair τ1 τ2).
+
+Derive Signature NoConfusion for Pat.
+
+End Pat.
